lib/zoo_saturn/spsc_bqueue.mli
@@ -3,6 +3,12 @@ type 'a t
 val create :
   int -> 'a t
 
+val size :
+  'a t -> int
+
+val is_empty :
+  'a t -> bool
+
 val push :
   'a t -> 'a -> bool
 
